%%%%%%%%%%%%%%%%%%%%%%%%%%%%%%%%%%%%%%%%%%%%%%%%%%%%%%%%%%%%%%%%%%%%%%%%%%%%%%%%%%%%%%%%%%%%%%%%%%%%%%%%%%%%%%%%%%%%%%%%%%%%%%%%%%%%%%%%%%%%%%%%%%%%%%%%%%%%%%%%%%%
% Written By Michael Brodskiy
% Class: Analysis of Random Phenomena
% Professor: I. Salama
%%%%%%%%%%%%%%%%%%%%%%%%%%%%%%%%%%%%%%%%%%%%%%%%%%%%%%%%%%%%%%%%%%%%%%%%%%%%%%%%%%%%%%%%%%%%%%%%%%%%%%%%%%%%%%%%%%%%%%%%%%%%%%%%%%%%%%%%%%%%%%%%%%%%%%%%%%%%%%%%%%%

\include{Includes.tex}

\title{Homework 8}
\date{\today}
\author{Michael Brodskiy\\ \small Professor: I. Salama}

\begin{document}

\maketitle

\begin{enumerate}

  \item We may write the correlation coefficient as:

    $$\rho_{XY}=\frac{\text{Cov}(X,Y)}{\sqrt{\text{Var}(X)\text{Var}(Y)}}$$

    Given that $Y=X+2Z$, we obtain:

    $$\text{Cov}(X,Y)=\text{Cov}(X,X+2Z)$$

    We break this apart to get:

    $$\text{Cov}(X,X+2Z)=\text{Cov}(X,X)+2\text{Cov}(X,Z)$$
    $$\text{Cov}(X,X+2Z)=\text{Var}(X)+2\text{Cov}(X,Z)$$

    Additionally, we get:

    $$\text{Var}(Y)=\text{Var}(X+2Z)$$
    $$\text{Var}(X+2Z)=3\text{Var}(X)+4\text{Var}(Z)+8\text{Cov}(X,Z)$$

    Thus, the expression becomes:

    $$\rho_{XY}=\frac{\text{Var}(X)+2\text{Cov}(X,Z)}{\sqrt{\text{Var}(X)[3\text{Var}(X)+4\text{Var}(Z)+8\text{Cov}(X,Z)]}}$$

    The final step is to calculate the covariance between $X$ and $Z$. Since it is stated that the two are independent, we arrive at:

    $$\text{Cov}(X,Z)=0$$

    And thus:

    $$\rho_{XY}=\frac{\text{Var}(X)}{\sqrt{\text{Var}(X)[3\text{Var}(X)+4\text{Var}(Z)]}}$$

    We plug in our known values to get:

    $$\rho_{XY}=\frac{16}{\sqrt{16[3(16)+4(4)]}}$$
    $$\boxed{\rho_{XY}=\frac{1}{2}}$$

    Since the correlation coefficient is not zero, \underline{$X$ and $Y$ are not independent}.

    Now, given $W=2X-Z$, we want to find:

    $$E[W]=E[2X-Z]$$
    $$\text{Var}(W)=\text{Var}(2X-Z)$$
    $$\text{Cov}(W,Y)=\text{Cov}(2X-Z,X+2Z)$$

    For the expectation value, we simply decompose to get:

    $$E[W]=2E[X]-E[Z]$$
    $$E[W]=2(2)-1$$
    $$\boxed{E[W]=3}$$

    The variance can be expanded to get:

    $$\text{Var}(W)=4\text{Var}(X)+\text{Var}(Z)-4\cancel{\text{Cov}(X,Z)}$$
    $$\text{Var}(W)=4(16)+4$$
    $$\boxed{\text{Var}(W)=68}$$

    Finally, we find the covariance as:

    $$\text{Cov}(W,Y)=\text{Cov}(2X,X+2Z)-\text{Cov}(Z, X+2Z)$$
    $$\text{Cov}(W,Y)=2\text{Var}(X) + 3\text{Cov}(X,Z)-2\text{Var}(Z)$$

    Plugging in values, we get:

    $$\text{Cov}(W,Y)=2(16) + \cancel{3\text{Cov}(X,Z)}-2(4)$$
    $$\boxed{\text{Cov}(W,Y)=24}$$

  \item

    \begin{enumerate}

      \item 

      \item 

      \item 

    \end{enumerate}

  \item

    \begin{enumerate}

      \item 

      \item 

      \item 

    \end{enumerate}

  \item

  \item

    \begin{enumerate}

      \item 

      \item 

      \item 

      \item 

      \item 

      \item 

      \item 

    \end{enumerate}

    \setcounter{enumi}{4}

  \item \textbf{Extra Credit}

    \begin{enumerate}

      \item 

      \item 

      \item 

      \item 

      \item 

      \item 

      \item 

    \end{enumerate}

  \item

    \begin{enumerate}

      \item 

      \item 

      \item 

      \item 

      \item 

      \item 

    \end{enumerate}

  \item

    \begin{enumerate}

      \item 

      \item 

    \end{enumerate}

  \item

  \item

\end{enumerate}

\end{document}

